deps/poulet4/lib/P4automata/WP.v
@@ -27,136 +27,32 @@ Section WeakestPre.
 
   Variable (a: P4A.t S H).
 
-  Definition expr_to_bit_expr (s: side) (e: P4A.expr H) : bit_expr H :=
+  Definition expr_to_bit_expr {c} (s: side) (e: P4A.expr H) : bit_expr H c :=
     match e with
-    | P4A.EHdr h => BEHdr s h
-    | P4A.ELit _ bs => BELit _ bs
+    | P4A.EHdr h => BEHdr c s h
+    | P4A.ELit _ bs => BELit _ c bs
     end.
 
-  Definition val_to_bit_expr (value: P4A.v) : bit_expr H :=
+  Definition val_to_bit_expr {c} (value: P4A.v) : bit_expr H c :=
     match value with
-    | P4A.VBits bs => BELit _ bs
+    | P4A.VBits bs => BELit _ c bs
     end.
 
-  Definition case_cond (cond: bit_expr H) (st': P4A.state_ref S) (s: P4A.sel_case S) :=
-    if st' == P4A.sc_st s
-    then BREq cond (val_to_bit_expr (P4A.sc_val s))
-    else BRFalse _.
-
-  Definition cases_cond (cond: bit_expr H) (st': P4A.state_ref S) (s: list (P4A.sel_case S)) :=
-    List.fold_right (@BROr H) (BRFalse _) (List.map (case_cond cond st') s).
-
-  Fixpoint case_negated_conds (cond: bit_expr H) (s: list (P4A.sel_case S)) :=
-    match s with
-    | nil => BRTrue _
-    | s :: rest =>
-      BRAnd
-        (BRNotEq cond (val_to_bit_expr (P4A.sc_val s)))
-        (case_negated_conds cond rest)
-    end.
-
-  Definition trans_cond (s: side) (t: P4A.transition S H) (st': P4A.state_ref S) :=
-    match t with
-    | P4A.TGoto _ r =>
-      if r == st'
-      then BRTrue _
-      else BRFalse _
-    | P4A.TSel cond cases default =>
-      let be_cond := expr_to_bit_expr s cond in
-      BROr (cases_cond be_cond st' cases)
-           (if default == st'
-            then case_negated_conds be_cond cases
-            else BRFalse _)
-    end.
-
-  Fixpoint bit_expr_subst (s: side) (h: P4A.hdr_ref H) (exp: bit_expr H) (phi: bit_expr H) : bit_expr H :=
-    match phi with
-    | BELit _ _
-    | BEBuf _ _ => phi
-    | BEHdr s' h' =>
-      if andb (s ==b s') (h ==b h')
-      then exp
-      else phi
-    | BESlice e hi lo =>
-      BESlice (bit_expr_subst s h exp e) hi lo
-    | BEConcat e1 e2 =>
-      BEConcat (bit_expr_subst s h exp e1)
-               (bit_expr_subst s h exp e2)
-    end.
-
-  Fixpoint store_rel_subst (s: side) (h: P4A.hdr_ref H) (exp: bit_expr H) (phi: store_rel H) : store_rel H :=
-    match phi with
-    | BRTrue _
-    | BRFalse _ =>
-      phi
-    | BREq e1 e2 =>
-      BREq (bit_expr_subst s h exp e1)
-           (bit_expr_subst s h exp e2)
-    | BRNotEq e1 e2 =>
-      BRNotEq (bit_expr_subst s h exp e1)
-              (bit_expr_subst s h exp e2)
-    | BRAnd r1 r2 =>
-      BRAnd (store_rel_subst s h exp r1)
-            (store_rel_subst s h exp r2)
-    | BROr r1 r2 =>
-      BROr (store_rel_subst s h exp r1)
-           (store_rel_subst s h exp r2)
-    | BRImpl r1 r2 =>
-      BRImpl (store_rel_subst s h exp r1)
-             (store_rel_subst s h exp r2)
-    end.
-
-  Fixpoint wp_op' (s: side) (o: P4A.op H) : nat * store_rel H -> nat * store_rel H :=
-    fun '(buf_idx, phi) =>
-      match o with
-      | P4A.OpNil _ => (buf_idx, phi)
-      | P4A.OpSeq o1 o2 =>
-        wp_op' s o1 (wp_op' s o2 (buf_idx, phi))
-      | P4A.OpExtract width hdr =>
-        let new_idx := buf_idx + width - 1 in
-        let slice := BESlice (BEBuf _ s) new_idx buf_idx in
-        (new_idx, store_rel_subst s hdr slice phi)
-      | P4A.OpAsgn lhs rhs =>
-        (buf_idx, store_rel_subst s lhs (expr_to_bit_expr s rhs) phi)
-      end.
-
-  Definition wp_op (s: side) (o: P4A.op H) (phi: store_rel H) : store_rel H :=
-    snd (wp_op' s o (0, phi)).
-
-  Inductive pred :=
-  | PredRead (s: state_template S)
-  | PredJump (cond: store_rel H) (s: S).
-
-  Definition pick_template (s: side) (c: conf_state S) : state_template S :=
-    match s with
-    | Left => c.(cs_st1)
-    | Right => c.(cs_st2)
-    end.
-
-  Definition preds (si: side) (candidates: list S) (s: state_template S) : list pred :=
-    if s.(st_buf_len) == 0
-    then [PredRead {| st_state := s.(st_state); st_buf_len := s.(st_buf_len) - 1 |}]
-    else List.map (fun candidate =>
-                     let st := a.(P4A.t_states) candidate in
-                     PredJump (trans_cond si (P4A.st_trans st) s.(st_state)) candidate)
-                  candidates.
-
-  Set Printing All.
-
-  Fixpoint be_subst (be: bit_expr H) (e: bit_expr H) (x: bit_expr H) : bit_expr H :=
+  Fixpoint be_subst {c} (be: bit_expr H c) (e: bit_expr H c) (x: bit_expr H c) : bit_expr H c :=
     match be with
-    | BELit _ l => BELit _ l
-    | BEBuf _ _
-    | BEHdr _ _ =>
+    | BELit _ _ l => BELit _ _ l
+    | BEBuf _ _ _
+    | BEHdr _ _ _
+    | BEVar _ _ =>
       if bit_expr_eq_dec a be x then e else be
     | BESlice be hi lo => BESlice (be_subst be e x) hi lo
     | BEConcat e1 e2 => BEConcat (be_subst e1 e x) (be_subst e2 e x)
     end.
 
-  Fixpoint sr_subst (sr: store_rel H) (e: bit_expr H) (x: bit_expr H) : store_rel H :=
+  Fixpoint sr_subst {c} (sr: store_rel H c) (e: bit_expr H c) (x: bit_expr H c) : store_rel H c :=
   match sr with
-  | BRTrue _ => BRTrue _
-  | BRFalse _ => BRFalse _
+  | BRTrue _ _
+  | BRFalse _ _ => sr
   | BREq e1 e2 => BREq (be_subst e1 e x) (be_subst e2 e x)
   | BRNotEq e1 e2 => BRNotEq (be_subst e1 e x) (be_subst e2 e x)
   | BRAnd r1 r2 => BRAnd (sr_subst r1 e x) (sr_subst r2 e x)
@@ -164,36 +60,107 @@ Section WeakestPre.
   | BRImpl r1 r2 => BRImpl (sr_subst r1 e x) (sr_subst r2 e x)
   end.
 
-  Definition wp_pred (si: side) (b: bool) (p: pred) (c: store_rel H) : store_rel H :=
-    let phi := sr_subst c (BEConcat (BEBuf _ si) (BELit _ [b])) (BEBuf _ si) in
-    match p with
-    | PredRead s =>
-      phi
-    | PredJump cond s =>
-      BRImpl cond
-             (wp_op si (a.(P4A.t_states) s).(P4A.st_op) phi)
+  Definition case_cond {c} (cond: bit_expr H c) (st': P4A.state_ref S) (s: P4A.sel_case S) :=
+    if st' == P4A.sc_st s
+    then BREq cond (val_to_bit_expr (P4A.sc_val s))
+    else BRFalse _ _.
+
+  Definition cases_cond {c} (cond: bit_expr H c) (st': P4A.state_ref S) (s: list (P4A.sel_case S)) :=
+    List.fold_right (@BROr _ _) (BRFalse _ _) (List.map (case_cond cond st') s).
+
+  Fixpoint case_negated_conds {c} (cond: bit_expr H c) (s: list (P4A.sel_case S)) : store_rel H c :=
+    match s with
+    | nil => BRTrue _ _
+    | s :: rest =>
+      BRAnd
+        (BRNotEq cond (val_to_bit_expr (P4A.sc_val s)))
+        (case_negated_conds cond rest)
     end.
 
-  Definition st_pred (p: pred) :=
+  Definition trans_cond
+             {c: bctx}
+             (s: side)
+             (t: P4A.transition S H)
+             (st': P4A.state_ref S)
+    : store_rel H c :=
+    match t with
+    | P4A.TGoto _ r =>
+      if r == st'
+      then BRTrue _ _
+      else BRFalse _ _
+    | P4A.TSel cond cases default =>
+      let be_cond := expr_to_bit_expr s cond in
+      BROr (cases_cond be_cond st' cases)
+           (if default == st'
+            then case_negated_conds be_cond cases
+            else BRFalse _ _)
+    end.
+
+  Fixpoint wp_op' {c} (s: side) (o: P4A.op H) : nat * store_rel H c -> nat * store_rel H c :=
+    fun '(buf_idx, phi) =>
+      match o with
+      | P4A.OpNil _ => (buf_idx, phi)
+      | P4A.OpSeq o1 o2 =>
+        wp_op' s o1 (wp_op' s o2 (buf_idx, phi))
+      | P4A.OpExtract width hdr =>
+        let new_idx := buf_idx + width - 1 in
+        let slice := BESlice (BEBuf _ _ s) new_idx buf_idx in
+        (new_idx, sr_subst phi (BEHdr _ s hdr) slice)
+      | P4A.OpAsgn lhs rhs =>
+        (buf_idx, sr_subst phi (BEHdr _ s lhs) (expr_to_bit_expr s rhs))
+      end.
+
+  Definition wp_op {c} (s: side) (o: P4A.op H) (phi: store_rel H c) : store_rel H c :=
+    snd (wp_op' s o (0, phi)).
+
+  Inductive pred (c: bctx) :=
+  | PredRead (s: state_template S)
+  | PredJump (cond: store_rel H c) (s: S).
+
+  Definition pick_template (s: side) (c: conf_state S) : state_template S :=
+    match s with
+    | Left => c.(cs_st1)
+    | Right => c.(cs_st2)
+    end.
+
+  Definition preds {c} (si: side) (candidates: list S) (s: state_template S) : list (pred c) :=
+    if s.(st_buf_len) == 0
+    then [PredRead _ {| st_state := s.(st_state); st_buf_len := s.(st_buf_len) - 1 |}]
+    else List.map (fun candidate =>
+                     let st := a.(P4A.t_states) candidate in
+                     PredJump (trans_cond si (P4A.st_trans st) s.(st_state)) candidate)
+                  candidates.
+
+  Definition wp_pred {c: bctx} (si: side) (b: bool) (p: pred c) (phi: store_rel H c) : store_rel H c :=
+    let phi' := sr_subst phi (BEConcat (BEBuf _ _ si) (BELit _ _ [b])) (BEBuf _ _ si) in
     match p with
-    | PredRead s => s
+    | PredRead _ s =>
+      phi'
+    | PredJump cond s =>
+      BRImpl cond
+             (wp_op si (a.(P4A.t_states) s).(P4A.st_op) phi')
+    end.
+
+  Definition st_pred {c} (p: pred c) :=
+    match p with
+    | PredRead _ s => s
     | PredJump _ s => {| st_state := inl s; st_buf_len := 0 |}
     end.
 
-  Definition wp_pred_pair (c: conf_rel S H) (preds: pred * pred) : list (conf_rel S H) :=
+  Definition wp_pred_pair {c} (phi: conf_rel S H c) (preds: pred c * pred c) : list (conf_rel S H c) :=
     let '(sl, sr) := preds in
     [{| cr_st := {| cs_st1 := st_pred sl;
                     cs_st2 := st_pred sr |};
-        cr_rel := wp_pred Left false sl (wp_pred Right false sr c.(cr_rel)) |};
+        cr_rel := wp_pred Left false sl (wp_pred Right false sr phi.(cr_rel)) |};
      {| cr_st := {| cs_st1 := st_pred sl;
                     cs_st2 := st_pred sr |};
-        cr_rel := wp_pred Left false sl (wp_pred Right false sr c.(cr_rel)) |}].
+        cr_rel := wp_pred Left true sl (wp_pred Right true sr phi.(cr_rel)) |}].
      
-  Definition wp (c: conf_rel S H) : list (conf_rel S H) :=
-    let cur_st_left  := c.(cr_st).(cs_st1) in
-    let cur_st_right := c.(cr_st).(cs_st2) in
+  Definition wp {c} (phi: conf_rel S H c) : list (conf_rel S H c) :=
+    let cur_st_left  := phi.(cr_st).(cs_st1) in
+    let cur_st_right := phi.(cr_st).(cs_st2) in
     let pred_pairs := list_prod (preds Left (List.map inl (enum S1)) cur_st_left)
                                 (preds Right (List.map inr (enum S2)) cur_st_right) in
-    List.concat (List.map (wp_pred_pair c) pred_pairs).
+    List.concat (List.map (wp_pred_pair phi) pred_pairs).
 
 End WeakestPre.
